Added predicate EveryPrepareClientOpMatchesRecordedPrePrepare to Inv.
With this predicate added to the Invariant we preserve the knowledge
that replicas vote with Prepare only for the first PrePrepare they have
received and stored from the Primary.
Debugging code removed as the proof now passes correctly.

docs/sbft-formal-model/proof.dfy
@@ -217,6 +217,21 @@ module Proof {
              && commitMsg.payload.operationWrapper == recordedPrePrepare.value.payload.operationWrapper)
   }
 
+  predicate {:opaque} EveryPrepareClientOpMatchesRecordedPrePrepare(c:Constants, v:Variables) {
+    && v.WF(c)
+    && (forall prepareMsg | && prepareMsg in v.network.sentMsgs
+                           && prepareMsg.payload.Prepare?
+                           && IsHonestReplica(c, prepareMsg.sender)
+                           && var replicaVariables := v.hosts[prepareMsg.sender].replicaVariables;
+                           && var replicaConstants := c.hosts[prepareMsg.sender].replicaConstants;
+                           && prepareMsg.payload.seqID in replicaVariables.workingWindow.getActiveSequenceIDs(replicaConstants)
+                           && prepareMsg.payload.view == replicaVariables.view
+          :: && var recordedPrePrepare := 
+                v.hosts[prepareMsg.sender].replicaVariables.workingWindow.prePreparesRcvd[prepareMsg.payload.seqID];
+             && recordedPrePrepare.Some?
+             && prepareMsg.payload.operationWrapper == recordedPrePrepare.value.payload.operationWrapper)
+  }
+
   predicate RecordedPreparesMatchHostView(c:Constants, v:Variables) {
     && v.WF(c)
     && (forall observer, seqID, sender | 
@@ -279,6 +294,7 @@ module Proof {
     && EveryCommitIsSupportedByPreviouslySentPrepares(c, v)
     && EverySentIntraViewMsgIsInWorkingWindowOrBefore(c, v)
     && EverySentIntraViewMsgIsForAViewLessOrEqualToSenderView(c, v)
+    && EveryPrepareClientOpMatchesRecordedPrePrepare(c, v)
     && EveryCommitClientOpMatchesRecordedPrePrepare(c, v)
     && HonestReplicasLockOnPrepareForGivenView(c, v)
     && HonestReplicasLockOnCommitForGivenView(c, v)
@@ -463,6 +479,7 @@ module Proof {
     requires NextStep(c, v, v', step)
     ensures RecordedCommitsClientOpsMatchPrePrepare(c, v')
     ensures EveryCommitIsSupportedByPreviouslySentPrepares(c, v')
+    ensures EveryPrepareClientOpMatchesRecordedPrePrepare(c, v')
     ensures EveryCommitClientOpMatchesRecordedPrePrepare(c, v')
     ensures HonestReplicasLockOnCommitForGivenView(c, v')
     ensures EveryCommitMsgIsSupportedByAQuorumOfPrepares(c, v')
@@ -471,57 +488,10 @@ module Proof {
     ProofEveryCommitMsgIsSupportedByAQuorumOfPrepares(c, v, v', step);
     reveal_RecordedCommitsClientOpsMatchPrePrepare();
     reveal_EveryCommitIsSupportedByPreviouslySentPrepares();
+    reveal_EveryPrepareClientOpMatchesRecordedPrePrepare();
     reveal_EveryCommitClientOpMatchesRecordedPrePrepare();
     reveal_HonestReplicasLockOnCommitForGivenView();
     ProofCommitMsgsFromHonestSendersAgree(c, v, v', step);
-    assert EveryCommitClientOpMatchesRecordedPrePrepare(c, v') by {
-      if (c.clusterConfig.IsHonestReplica(step.id)) {
-        var h_c := c.hosts[step.id].replicaConstants;
-        var h_v := v.hosts[step.id].replicaVariables;
-        var h_v' := v'.hosts[step.id].replicaVariables;
-        var h_step :| Replica.NextStep(h_c, h_v, h_v', step.msgOps, h_step);
-        if(h_step.SendPrePrepareStep?) {
-          assert EveryCommitClientOpMatchesRecordedPrePrepare(c, v');
-        } else if(h_step.RecvPrePrepareStep?) {
-          assert EveryCommitClientOpMatchesRecordedPrePrepare(c, v');
-        } else if(h_step.SendPrepareStep?) {
-          assert EveryCommitClientOpMatchesRecordedPrePrepare(c, v');
-        } else if(h_step.RecvPrepareStep?) {
-          assert EveryCommitClientOpMatchesRecordedPrePrepare(c, v');
-        } else if(h_step.SendCommitStep?) {
-          assert EveryCommitClientOpMatchesRecordedPrePrepare(c, v');
-        } else if(h_step.RecvCommitStep?) {
-          assert EveryCommitClientOpMatchesRecordedPrePrepare(c, v');
-        } else if(h_step.DoCommitStep?) {
-          assert EveryCommitClientOpMatchesRecordedPrePrepare(c, v');
-        } else if(h_step.ExecuteStep?) {
-          assert EveryCommitClientOpMatchesRecordedPrePrepare(c, v');
-        } else if(h_step.SendCheckpointStep?) {
-          assert EveryCommitClientOpMatchesRecordedPrePrepare(c, v');
-        } else if(h_step.RecvCheckpointStep?) {
-          assert EveryCommitClientOpMatchesRecordedPrePrepare(c, v');
-        } else if(h_step.AdvanceWorkingWindowStep?) {
-          assert EveryCommitClientOpMatchesRecordedPrePrepare(c, v');
-        } else if(h_step.PerformStateTransferStep?) {
-          assert EveryCommitClientOpMatchesRecordedPrePrepare(c, v');
-        } else if(h_step.LeaveViewStep?) {
-          assert EveryCommitClientOpMatchesRecordedPrePrepare(c, v');
-        } else if(h_step.SendViewChangeMsgStep?) {
-          assert EveryCommitClientOpMatchesRecordedPrePrepare(c, v');
-        } else if(h_step.RecvViewChangeMsgStep?) {
-          assert EveryCommitClientOpMatchesRecordedPrePrepare(c, v');
-        } else if(h_step.SelectQuorumOfViewChangeMsgsStep?) {
-          assert EveryCommitClientOpMatchesRecordedPrePrepare(c, v');
-        } else if(h_step.SendNewViewMsgStep?) {
-          assert EveryCommitClientOpMatchesRecordedPrePrepare(c, v');
-        } else if(h_step.RecvNewViewMsgStep?) {
-          assert EveryCommitClientOpMatchesRecordedPrePrepare(c, v');
-        }
-        else {
-          assert EveryCommitClientOpMatchesRecordedPrePrepare(c, v');
-        }
-      }
-    }
   }
 
   lemma QuorumOfPreparesInNetworkMonotonic(c: Constants, v:Variables, v':Variables, step:Step)
@@ -675,6 +645,7 @@ module Proof {
     requires SendPrepareIsEnabled(c, v, v', step, h_step)
     ensures Inv(c, v')
   {
+    reveal_EveryPrepareClientOpMatchesRecordedPrePrepare();
     CommitMsgStability(c, v, v', step);
   }
 
@@ -1117,6 +1088,7 @@ module Proof {
     if Init(c, v) {
       reveal_RecordedCommitsClientOpsMatchPrePrepare();
       reveal_EveryCommitIsSupportedByPreviouslySentPrepares();
+      reveal_EveryPrepareClientOpMatchesRecordedPrePrepare();
       reveal_EveryCommitClientOpMatchesRecordedPrePrepare();
       reveal_HonestReplicasLockOnCommitForGivenView();
       reveal_CommitMsgsFromHonestSendersAgree();
